src/tidy/rewrite_search/default.lean
@@ -1,7 +1,7 @@
 -- "init.lean" provides the fallback strategy and tracer for the engine.
 import .init
 
--- 'tactic.lean' provides the tactics
+-- "tactic.lean" provides the tactics
 import .tactic
 
 import .tracer
