src/tidy/rewrite_search/strategy/default.lean
@@ -1,1 +1,1 @@
-import .explore
+import .pexplore
