test/rewrite_search_vs_ring.lean
@@ -13,13 +13,13 @@ lemma test3 : (a * (b + c)) * d = a * (b * d) + a * (c * d) :=
 by rewrite_search [add_comm, add_assoc, mul_assoc, /-mul_comm,-/ left_distrib, right_distrib] {trace_result := tt, trace_summary := tt, /-view := visualiser,-/ metric := edit_distance}
 
 lemma test4 : (a * (b + c + 1)) * d = a * (b * d) + a * (1 * d) + a * (c * d) :=
-by rewrite_search [add_comm, add_assoc, mul_one, mul_assoc, /-mul_comm,-/ left_distrib, right_distrib] {trace_result := tt, trace_summary := tt, /-view := visualiser,-/ metric := edit_distance_cm_weighted 3, strategy := explore {max_iterations := 100}}
+by rewrite_search [add_comm, add_assoc, mul_one, mul_assoc, /-mul_comm,-/ left_distrib, right_distrib] {trace_result := tt, trace_summary := tt, /-view := visualiser,-/ metric := edit_distance_cm_weighted 3, strategy := pexplore {max_iterations := 100}}
 
 lemma test4_ring : (a * (b + c + 1)) * d = a * (b * d) + a * (1 * d) + a * (c * d) :=
 by ring
 
 lemma test5 : (a * (b + c + 1) / e) * d = a * (b / e * d) + a * (1 / e * d) + a * (c / e * d) :=
-by rewrite_search [add_comm, add_assoc, mul_one, mul_assoc, /-mul_comm,-/ left_distrib, right_distrib] {trace_result := tt, trace_summary := tt, /-view := visualiser,-/ metric := edit_distance_cm_weighted 3, strategy := explore {max_iterations := 500}}
+by rewrite_search [add_comm, add_assoc, mul_one, mul_assoc, /-mul_comm,-/ left_distrib, right_distrib] {trace_result := tt, trace_summary := tt, /-view := visualiser,-/ metric := edit_distance_cm_weighted 3, strategy := pexplore {max_iterations := 500}}
 
 lemma test5_ring : (a * (b + c + 1) / e) * d = a * (b / e * d) + a * (1 / e * d) + a * (c / e * d) :=
 by ring
